src/Typechecker/ClassTypechecker.v
@@ -1,0 +1,8 @@
+Require Import
+        FJ.Base
+        FJ.Syntax
+        FJ.Semantics.AuxiliarDefinitions
+        FJ.Typing
+        FJ.Tactics
+        FJ.Typechecker.ExpTypechecker
+        FJ.Typechecker.MethodTypechecker.
