src/Typechecker/ExpTypechecker.v
@@ -37,24 +37,21 @@ Definition ExpHasTypeDec
                  match m_type_lookupDec n CT C m with
                  | !! => ??
                  | [|| p ||] =>
-                   match p with
-                   | (Cs , t) =>
-                     match eq_nat_dec (length es) (length Cs) with
+                     match eq_nat_dec (length es) (length (mtparams p)) with
                      | Yes =>
                        match Forall_partial (ExpHasTypeDec n CT G) es with
                        | ?? => ??
                        | Found _ Ds _ =>
-                         match eq_nat_dec (length Ds) (length Cs) with
+                         match eq_nat_dec (length Ds) (length (mtparams p)) with
                          | Yes =>
-                           match Forall2_dec (BoundedSubtypeDec CT n) Ds Cs _ with
-                           | Yes => _
+                           match Forall2_dec (BoundedSubtypeDec CT n) Ds (mtparams p) _ with
+                           | Yes => Found _ (mttype p) _
                            | No => ??           
                            end
                          | No  => ??  
                          end
                        end  
-                     | No  => ??           
-                     end  
+                     | No  => ??            
                    end
                  end
                end                        
@@ -75,54 +72,29 @@ Definition ExpHasTypeDec
                    end
                  end  
                end                
-            | ENew C es => fun _ => _
+            | ENew C es => fun _ =>
+               match fieldsDec n CT C with
+               | !! => ??
+               | [|| fs ||] =>
+                 match eq_nat_dec (length es) (length (values fs)) with
+                 | No => ??
+                 | Yes =>
+                   match Forall_partial (ExpHasTypeDec n CT G) es with
+                   | ?? => ??
+                   | Found _ Ds _ =>
+                     match eq_nat_dec (length Ds) (length (map fdtype (values fs))) with
+                     | No => ??
+                     | Yes =>
+                       match Forall2_dec (BoundedSubtypeDec CT n) Ds
+                                         (map fdtype (values fs)) _ with
+                       | Yes => Found _ C _
+                       | No  => ??           
+                       end
+                     end
+                   end
+                 end
+               end
             end (eq_refl e)) ; clear ExpHasTypeDec ; simpl in * ; substs ; eauto ;
     try (intro C ; intro H ; inverts* H ; map_solver).
-  eapply BoundedSubtypeForall2 in f0 ; eauto.
-  destruct e3. destruct e0. destruct a.
-  eauto.
-
+  Defined.
   
-(*
-Definition ExpHasTypeDec
-  : forall (n : nat) CT G e, {C | CT ; G |-- e :: C} + {forall C, ~ (CT ; G |-- e :: C)}.
-  refine (fix ExpHasTypeDec n CT G e : {C | CT ; G |-- e :: C} +
-                                       {forall C, ~ (CT ; G |-- e :: C)} :=
-            match e as e'
-                  return e = e' -> {C | CT ; G |-- e :: C} + {forall C, ~ (CT ; G |-- e :: C)} with
-            | EVar v => fun _ =>
-               match MapsToDec v G with
-               | !! => !!
-               | [|| t ||] => [|| t ||]          
-               end          
-            | EFieldAccess e v => fun _ =>
-               match ExpHasTypeDec n CT G e with
-               | [|| C ||] =>
-                 match fieldsDec n CT C with
-                 | !! => !!
-                 | [|| fds ||] =>
-                   match MapsToDec v fds with
-                   | !! => !!
-                   | [|| ft ||] => [|| fdtype ft ||]          
-                   end
-                 end
-               | !! => !!  
-               end                      
-            | EMethodInvoc e m es => fun _ =>
-               match ExpHasTypeDec n CT G e with
-               | !! => !!
-               | [|| C ||] =>
-                 match m_type_lookupDec n CT C m with
-                 | !! => !!
-                 | [|| p ||] =>
-                   match p with
-                   | (Cs , t) => _
-                   end
-                 end
-               end                        
-            | ECast C e => fun _ => _
-            | ENew C es => fun _ => _                          
-            end (eq_refl e)) ; clear ExpHasTypeDec ; simpl in * ; substs ; eauto ;
-    try (intro C ; intro H ; inverts* H ; map_solver).
-    intro C1 ; intro H ; inverts H.
-*)
