src/Typechecker/MethodTypechecker.v
@@ -1,0 +1,32 @@
+Require Import
+        FJ.Base
+        FJ.Syntax
+        FJ.Semantics.AuxiliarDefinitions
+        FJ.Typing
+        FJ.Tactics
+        FJ.Typechecker.ExpTypechecker.
+
+
+Definition MethodOkDec : forall (n : nat) CT C (M : Method), {{ M | MethodOk CT C M}}.
+  refine (fun n CT C M =>
+            match MapsToDec C CT with
+            | !! => ??
+            | [|| CD ||] =>
+                match ExpHasTypeDec n CT (mkGamma ((mkFormalArg this C) :: (margs M)))
+                                    (mbody M) with
+                | ?? => ??
+                | Found _ D _ =>
+                  match valid_overrideDec CT n (mname M) (cextends CD)
+                                          (mkMethodType (map ftype (margs M)) (mtype M)) with
+                  | No => ??
+                  | Yes =>
+                    match BoundedSubtypeDec CT n D (mtype M) with
+                    | Yes => Found _ M _
+                    | No  => ??               
+                    end
+                  end   
+              end
+            end) ; simpl in * ; try map_solver ; eauto.
+  eapply T_Method ;eauto.
+  eapply BoundedSubtypeSound ; eauto.
+Defined.
